TM/Code/Copy.v
@@ -1,0 +1,215 @@
+(* Helper functions for verifying machines using CopySymbols and MoveToSymbol *)
+
+Require Import TM.Code.CodeTM.
+Require Import TM.Compound.CopySymbols TM.Compound.MoveToSymbol.
+
+Section Copy.
+
+  (*
+  Section Test.
+
+    Let inputX := encode (4, 3).
+    Compute inputX.
+
+    Let t : tape (Bool_Fin + Bool_Fin)^+ :=
+      midtape [inr START] (inl (inl true))
+              (map inl [inl true; inl true; inl true; inl false; 
+                          inr true; inr true; inr true; inr false] ++ [inr STOP; inl (inl true)]).
+
+    Compute tape_local t.
+    Let stop_X :=
+      fun (x : (Bool_Fin+Bool_Fin)^+) =>
+        match x with
+        | (inl (inl _)) => false
+        | _ => true (* Stop at symbol from Y or halt/stop symbol *)
+        end.
+
+    Ltac re x := assert (x = x) by reflexivity.
+
+    (* CopySymbols_Fun is not computable!  Use the equational rewriting to "execute"
+     * (CopSymbols_Fun can be made computable by changing the termination proof to Qed.)
+     *)
+    Goal True.
+      re (tape_local (fst (CopySymbols_Fun stop_X id (t, rightof (inr START) [])))).
+      re (snd (CopySymbols_Fun stop_X id (t, rightof (inr START) []))).
+      re ((left (snd (CopySymbols_Fun stop_X id (t, rightof (inr START) []))))).
+      subst t; repeat ( rewrite CopySymbols_Fun_equation in *; cbn in * ); cbv [id] in *.
+    Abort.
+
+
+    Goal True.
+      re (right (MoveToSymbol_Fun stop_X t)).
+      re (left (MoveToSymbol_Fun stop_X t)).
+      re (current (MoveToSymbol_Fun stop_X t)).
+      re (tape_local (MoveToSymbol_Fun stop_X t)).
+      Compute t.
+      subst t; repeat ( rewrite MoveToSymbol_Fun_equation in *; cbn in * ).
+    Abort.
+    
+  End Test.
+   *)
+  
+  Variable sig : finType.
+  Variable stop : sig -> bool.
+
+  Lemma CopySymbols_pair_first tltr str1 x str2 tl' tr':
+    (forall x, List.In x str1 -> stop x = false) ->
+    (stop x = true) ->
+    tape_local (fst tltr) = str1 ++ [x] ++ str2 ->
+    (tl', tr') = CopySymbols_Fun stop id tltr ->
+    tape_local tl' = x :: str2.
+  Proof.
+    intros H H0. destruct tltr as [tl tr]. intros H1 E0.
+    destruct tl as [ | r rs | l ls | ls m rs]; cbn in *.
+    1-3: rewrite CopySymbols_Fun_equation in E0; inv H1; exfalso; destruct str1; cbn in *; congruence.
+    revert rs tr ls H ls m H1 tl' tr' E0. revert str1; intros str1.
+    induction str1 as [ | s' str1' IHstr1]; (* cbn in *; *) intros.
+    - cbn in *. inv H1. rewrite CopySymbols_Fun_equation in E0. rewrite H0 in E0. inv E0. cbn. auto.
+    - rewrite CopySymbols_Fun_equation in E0. destruct (stop m) eqn:E1.
+      + inv E0. cbn in *. inv H1. enough (stop s' = false)  by congruence; eauto.
+      + cbn in H1. inv H1. cbn in *. destruct str1'; cbn in *; eapply IHstr1; eauto.
+  Qed.
+
+  Lemma CopySymbols_pair_second tltr str1 x str2 tl' tr':
+    (forall x, List.In x str1 -> stop x = false) ->
+    (stop x = true) ->
+    tape_local (fst tltr) = str1 ++ [x] ++ str2 ->
+    (tl', tr') = CopySymbols_Fun stop id tltr ->
+    left tr' = rev str1 ++ left (snd tltr).
+  Proof.
+    intros H H0. destruct tltr as [tl tr]. intros H1 E0.
+    destruct tl as [ | r rs | l ls | ls m rs]; cbn in *.
+    1-3: rewrite CopySymbols_Fun_equation in E0; inv H1; exfalso; destruct str1; cbn in *; congruence.
+    revert rs tr ls H ls m H1 tl' tr' E0. revert str1; intros str1.
+    induction str1 as [ | s' str1' IHstr1]; (* cbn in *; *) intros.
+    - cbn in *. inv H1. rewrite CopySymbols_Fun_equation in E0. rewrite H0 in E0. inv E0. cbn. auto.
+    - rewrite CopySymbols_Fun_equation in E0. destruct (stop m) eqn:E1.
+      + inv E0. cbn in *. inv H1. enough (stop s' = false)  by congruence; eauto.
+      + cbn in H1. inv H1. cbn in *.
+        simpl_list; cbn.
+        destruct str1'; cbn in *.
+        * clear H. erewrite IHstr1; eauto. destruct tr; cbn; eauto. destruct l0; cbn; auto.
+        * simpl_list; cbn.
+          erewrite IHstr1; eauto. destruct tr; simpl_list; cbn; eauto. destruct l0; cbn; auto.
+  Qed.
+
+
+  Lemma MoveToSymbol_right t str1 str2 x :
+    (forall x, List.In x str1 -> stop x = false) ->
+    (stop x = true) ->
+    tape_local t = str1 ++ x :: str2 ->
+    right (MoveToSymbol_Fun stop t) = str2 /\
+    current (MoveToSymbol_Fun stop t) = Some x.
+  Proof.
+    intros H H0. destruct t as [ | r rs | l ls | ls m rs]; cbn in *.
+    1,3: rewrite MoveToSymbol_Fun_equation; cbn; destruct str1; cbn in *; try congruence.
+    1: destruct str1; cbn in *; congruence.
+    revert m ls str1 H. revert rs.
+    refine (@size_induction _ (@length sig) _ _); intros [ | s rs'] IH; intros.
+    - rewrite MoveToSymbol_Fun_equation; cbn. destruct str1; cbn in *; inv H1.
+      + rewrite H0. cbn. auto.
+      + destruct str1; cbn in *; congruence.
+    - rewrite MoveToSymbol_Fun_equation; cbn.
+      destruct (stop m) eqn:E1.
+      + cbn. destruct str1; cbn in *; inv H1; eauto. specialize (H _ ltac:(eauto)). congruence.
+      + destruct str1; cbn in *; inv H1.
+        * congruence.
+        * eapply IH; cbn; eauto.
+  Qed.
+
+  Lemma MoveToSymbol_left t str1 str2 x :
+    (forall x, List.In x str1 -> stop x = false) ->
+    (stop x = true) ->
+    tape_local t = str1 ++ x :: str2 ->
+    left (MoveToSymbol_Fun stop t) = rev str1 ++ left t.
+  Proof.
+    intros H H0. destruct t as [ | r rs | l ls | ls m rs]; cbn in *.
+    1,3: rewrite MoveToSymbol_Fun_equation; cbn; destruct str1; cbn in *; try congruence.
+    1: destruct str1; cbn in *; congruence.
+    revert m ls str1 H. revert rs.
+    refine (@size_induction _ (@length sig) _ _); intros [ | s rs'] IH; intros.
+    - rewrite MoveToSymbol_Fun_equation; cbn. destruct str1; cbn in *; inv H1.
+      + rewrite H0. cbn. auto.
+      + destruct str1; cbn in *; congruence.
+    - rewrite MoveToSymbol_Fun_equation; cbn.
+      destruct (stop m) eqn:E1.
+      + cbn. destruct str1; cbn in *; inv H1; eauto. specialize (H _ ltac:(eauto)). congruence.
+      + destruct str1; cbn in *; inv H1.
+        * congruence.
+        * simpl_list. eapply IH; cbn; eauto.
+  Qed.
+
+  Corollary MoveToSymbol_L_left t str1 str2 x :
+    (forall x, List.In x str1 -> stop x = false) ->
+    (stop x = true) ->
+    tape_local_l t = str1 ++ x :: str2 ->
+    left (MoveToSymbol_L_Fun stop t) = str2 /\
+    current (MoveToSymbol_L_Fun stop t) = Some x.
+  Proof.
+    intros. pose proof (@MoveToSymbol_right (mirror_tape t) str1 str2 x) as L.
+    simpl_tape in L. repeat spec_assert L by auto. destruct L as (L1,L2).
+    erewrite (MoveToSymbol_mirror' (t' := mirror_tape (MoveToSymbol_L_Fun stop t))) in L1, L2; simpl_tape; eauto.
+    simpl_tape in *. auto.
+  Qed.
+
+  Corollary MoveToSymbol_L_right t str1 str2 x :
+    (forall x, List.In x str1 -> stop x = false) ->
+    (stop x = true) ->
+    tape_local_l t = str1 ++ x :: str2 ->
+    right (MoveToSymbol_L_Fun stop t) = rev str1 ++ right t.
+  Proof.
+    intros. pose proof (@MoveToSymbol_left (mirror_tape t) str1 str2 x) as L.
+    simpl_tape in L. repeat spec_assert L by auto.
+    erewrite (MoveToSymbol_mirror' (t' := mirror_tape (MoveToSymbol_L_Fun stop t))) in L; simpl_tape; eauto.
+    simpl_tape in *. auto.
+  Qed.
+
+
+  (* Termination times *)
+
+  (* The termination times of CopySymbols and MoveTosymbol only differ in the factors *)
+
+  Lemma CopySymbols_TermTime_local t r1 sym r2 :
+    tape_local t = r1 ++ sym :: r2 ->
+    stop sym = true ->
+    CopySymbols_TermTime stop t <= 8 + 8 * length r1.
+  Proof.
+    revert t sym r2. induction r1; intros t sym r2 HEnc HStop; cbn -[plus mult] in *.
+    - destruct t; cbn in HEnc; inv HEnc. rewrite CopySymbols_TermTime_equation. rewrite HStop. cbn. omega.
+    - destruct t; cbn in HEnc; try congruence. inv HEnc.
+      rewrite CopySymbols_TermTime_equation. destruct (stop a).
+      + omega.
+      + apply Nat.add_le_mono_l. replace (8 * S (|r1|)) with (8 + 8 * |r1|) by omega.
+        eapply IHr1; eauto. cbn. now simpl_tape.
+  Qed.
+
+  Lemma MoveToSymbols_TermTime_local t r1 sym r2 :
+    tape_local t = r1 ++ sym :: r2 ->
+    stop sym = true ->
+    MoveToSymbol_TermTime stop t <= 4 + 4 * length r1.
+  Proof.
+    revert t sym r2. induction r1; intros t sym r2 HEnc HStop; cbn -[plus mult] in *.
+    - destruct t; cbn in HEnc; inv HEnc. rewrite MoveToSymbol_TermTime_equation. rewrite HStop. cbn. omega.
+    - destruct t; cbn in HEnc; try congruence. inv HEnc.
+      rewrite MoveToSymbol_TermTime_equation. destruct (stop a).
+      + omega.
+      + apply Nat.add_le_mono_l. replace (4 * S (|r1|)) with (4 + 4 * |r1|) by omega.
+        eapply IHr1; eauto. cbn. now simpl_tape.
+  Qed.
+
+
+  Lemma MoveToSymbols_TermTime_local_l t r1 sym r2 :
+    tape_local_l t = r1 ++ sym :: r2 ->
+    stop sym = true ->
+    MoveToSymbol_L_TermTime stop t <= 4 + 4 * length r1.
+  Proof.
+    revert t sym r2. induction r1; intros t sym r2 HEnc HStop; cbn -[plus mult] in *.
+    - destruct t; cbn in HEnc; inv HEnc. rewrite MoveToSymbol_L_TermTime_equation. rewrite HStop. cbn. omega.
+    - destruct t; cbn in HEnc; try congruence. inv HEnc.
+      rewrite MoveToSymbol_L_TermTime_equation. destruct (stop a).
+      + omega.
+      + apply Nat.add_le_mono_l. replace (4 * S (|r1|)) with (4 + 4 * |r1|) by omega.
+        eapply IHr1; eauto. cbn. now simpl_tape.
+  Qed.
+  
+End Copy.
